src/Lustre/LSemantics.v
@@ -11,6 +11,7 @@ From Velus Require Import Environment.
 From Velus Require Import Operators.
 From Velus Require Import Clocks.
 From Velus Require Import Lustre.LSyntax.
+From Velus Require Import Streams.
 
 (** * Lustre semantics *)
 
@@ -20,21 +21,13 @@ Module Type LSEMANTICS
        (Import OpAux : OPERATORS_AUX Op)
        (Import Syn   : LSYNTAX   Ids Op).
 
-  (* TODO: put this somewhere else *)
-  Infix ":::" := Cons (at level 60, right associativity) : stream_scope.
-  Delimit Scope stream_scope with Stream.
-  Open Scope stream_scope.
-
   Definition history := Env.t (Stream value).
 
-  CoFixpoint const (c: const) (b: Stream bool) : Stream value :=
-    match b with
-    | true  ::: b' => present (sem_const c) ::: const c b'
-    | false ::: b' => absent ::: const c b'
-    end.
+  CoFixpoint const (c: const) (b: Stream bool): Stream value :=
+    (if hd b then present (sem_const c) else absent) ::: const c (tl b).
 
   CoInductive lift1 (op: unop) (ty: type)
-                                     : Stream value -> Stream value -> Prop :=
+    : Stream value -> Stream value -> Prop :=
   | Lift1A:
       forall xs rs,
         lift1 op ty xs rs ->
@@ -46,7 +39,7 @@ Module Type LSEMANTICS
         lift1 op ty (present x ::: xs) (present r ::: rs).
 
   CoInductive lift2 (op: binop) (ty1 ty2: type)
-                      : Stream value -> Stream value -> Stream value -> Prop :=
+    : Stream value -> Stream value -> Stream value -> Prop :=
   | Lift2A:
       forall xs ys rs,
         lift2 op ty1 ty2 xs ys rs ->
@@ -58,7 +51,7 @@ Module Type LSEMANTICS
         lift2 op ty1 ty2 (present x ::: xs) (present y ::: ys) (present r ::: rs).
 
   CoInductive fby1
-               : val -> Stream value -> Stream value -> Stream value -> Prop :=
+    : val -> Stream value -> Stream value -> Stream value -> Prop :=
   | Fby1A:
       forall v xs ys rs,
         fby1 v xs ys rs ->
@@ -79,24 +72,24 @@ Module Type LSEMANTICS
         fby (present x ::: xs) (present y ::: ys) (present x ::: rs).
 
   CoInductive when (k: bool)
-                       : Stream value -> Stream value -> Stream value -> Prop :=
+    : Stream value -> Stream value -> Stream value -> Prop :=
   | WhenA:
       forall xs cs rs,
-        when k xs cs rs ->
+        when k cs xs rs ->
         when k (absent ::: cs) (absent ::: xs) (absent ::: rs)
   | WhenPA:
       forall x c xs cs rs,
-        when k xs cs rs ->
+        when k cs xs rs ->
         val_to_bool c = Some (negb k) ->
         when k (present c ::: cs) (present x ::: xs) (absent ::: rs)
   | WhenPP:
       forall x c xs cs rs,
-        when k xs cs rs ->
+        when k cs xs rs ->
         val_to_bool c = Some k ->
         when k (present c ::: cs) (present x ::: xs) (present x ::: rs).
 
   CoInductive merge
-       : Stream value -> Stream value -> Stream value -> Stream value -> Prop :=
+    : Stream value -> Stream value -> Stream value -> Stream value -> Prop :=
   | MergeA:
       forall xs ts fs rs,
         merge xs ts fs rs ->
@@ -113,7 +106,7 @@ Module Type LSEMANTICS
               (absent ::: ts) (present f ::: fs) (present f ::: rs).
 
   CoInductive ite
-       : Stream value -> Stream value -> Stream value -> Stream value -> Prop :=
+    : Stream value -> Stream value -> Stream value -> Stream value -> Prop :=
   | IteA:
       forall s ts fs rs,
         ite s ts fs rs ->
@@ -122,12 +115,12 @@ Module Type LSEMANTICS
       forall t f s ts fs rs,
         ite s ts fs rs ->
         ite (present true_val ::: s)
-              (present t ::: ts) (present f ::: fs) (present t ::: rs)
+            (present t ::: ts) (present f ::: fs) (present t ::: rs)
   | IteF:
       forall t f s ts fs rs,
         ite s ts fs rs ->
         ite (present false_val ::: s)
-              (present t ::: ts) (present f ::: fs) (present f ::: rs).
+            (present t ::: ts) (present f ::: fs) (present f ::: rs).
 
   Definition sclockof xs := map (fun x => x <> absent) xs.
 
@@ -138,14 +131,28 @@ Module Type LSEMANTICS
   (* TODO: replace idents with (list ident) *)
   Definition idents xs := List.map (@fst ident (type * clock)) xs.
 
-  Notation sem_var H := (fun (x: ident) (s: Stream value) => Env.MapsTo x s H).
+  Inductive sem_var: history -> ident -> Stream value -> Prop :=
+    sem_var_intro:
+      forall H x xs xs',
+        Env.find x H = Some xs' ->
+        xs ≡ xs' ->
+        sem_var H x xs.
+
+  CoInductive reset_of: Stream value -> Stream bool -> Prop :=
+    reset_of_intro:
+      forall v vs b bs,
+        reset_of vs bs ->
+        value_to_bool v = Some b ->
+        reset_of (v ::: vs) (b ::: bs).
+
+  Definition mask_v := mask absent.
 
   Section NodeSemantics.
 
     Variable G : global.
 
     Inductive sem_exp
-               : history -> Stream bool -> exp -> list (Stream value) -> Prop :=
+      : history -> Stream bool -> exp -> list (Stream value) -> Prop :=
     | Sconst:
         forall H b c,
           sem_exp H b (Econst c) [const c b]
@@ -205,24 +212,39 @@ Module Type LSEMANTICS
         forall H b f es lann ss os,
           Forall2 (sem_exp H b) es ss ->
           sem_node f (concat ss) os ->
-          sem_exp H b (Eapp f es lann) os
+          sem_exp H b (Eapp f es None lann) os
+
+    | Sreset:
+        forall H b f es r lann ss os rs bs,
+          Forall2 (sem_exp H b) es ss ->
+          sem_exp H b r [rs] ->
+          reset_of rs bs ->
+          sem_reset f bs (concat ss) os ->
+          sem_exp H b (Eapp f es (Some r) lann) os
 
     with sem_equation: history -> Stream bool -> equation -> Prop :=
-    | Seq:
-        forall H b xs es ss,
-          Forall2 (sem_exp H b) es ss ->
-          Forall2 (sem_var H) xs (concat ss) ->
-          sem_equation H b (xs, es)
+           Seq:
+             forall H b xs es ss,
+               Forall2 (sem_exp H b) es ss ->
+               Forall2 (sem_var H) xs (concat ss) ->
+               sem_equation H b (xs, es)
 
     with sem_node: ident -> list (Stream value) -> list (Stream value) -> Prop :=
-    | Snode:
-        forall f ss os n H b,
-          find_node f G = Some n ->
-          Forall2 (sem_var H) (idents n.(n_in)) ss ->
-          Forall2 (sem_var H) (idents n.(n_out)) os ->
-          Forall (sem_equation H b) n.(n_eqs) ->
-          b = sclocksof ss ->
-          sem_node f ss os.
+           Snode:
+             forall f ss os n H b,
+               find_node f G = Some n ->
+               Forall2 (sem_var H) (idents n.(n_in)) ss ->
+               Forall2 (sem_var H) (idents n.(n_out)) os ->
+               Forall (sem_equation H b) n.(n_eqs) ->
+               b = sclocksof ss ->
+               sem_node f ss os
+
+    with sem_reset: ident -> Stream bool -> list (Stream value) -> list (Stream value) -> Prop :=
+           SReset:
+             forall f r xss yss,
+               (forall k, sem_node f (List.map (mask_v k r) xss) (List.map (mask_v k r) yss)) ->
+               sem_reset f r xss yss.
+
 
   End NodeSemantics.
 
@@ -239,6 +261,7 @@ Module Type LSEMANTICS
     Variable P_exp : history -> Stream bool -> exp -> list (Stream value) -> Prop.
     Variable P_equation : history -> Stream bool -> equation -> Prop.
     Variable P_node : ident -> list (Stream value) -> list (Stream value) -> Prop.
+    Variable P_reset : ident -> Stream bool -> list (Stream value) -> list (Stream value) -> Prop.
 
     Hypothesis ConstCase:
       forall H b c,
@@ -312,7 +335,18 @@ Module Type LSEMANTICS
         Forall2 (P_exp H b) es ss ->
         sem_node G f (concat ss) os ->
         P_node f (concat ss) os ->
-        P_exp H b (Eapp f es lann) os.
+        P_exp H b (Eapp f es None lann) os.
+
+    Hypothesis ResetCase:
+      forall H b f es r lann ss os rs bs,
+        Forall2 (sem_exp G H b) es ss ->
+        Forall2 (P_exp H b) es ss ->
+        sem_exp G H b r [rs] ->
+        P_exp H b r [rs] ->
+        reset_of rs bs ->
+        sem_reset G f bs (concat ss) os ->
+        P_reset f bs (concat ss) os ->
+        P_exp H b (Eapp f es (Some r) lann) os.
 
     Hypothesis Equation:
       forall H b xs es ss,
@@ -330,6 +364,12 @@ Module Type LSEMANTICS
         Forall (P_equation H b) n.(n_eqs) ->
         b = sclocksof ss ->
         P_node f ss os.
+
+    Hypothesis Reset:
+      forall f r xss yss,
+        (forall k, sem_node G f (List.map (mask_v k r) xss) (List.map (mask_v k r) yss)
+              /\ P_node f (List.map (mask_v k r) xss) (List.map (mask_v k r) yss)) ->
+        P_reset f r xss yss.
 
     Local Ltac SolveForall :=
       match goal with
@@ -354,23 +394,27 @@ Module Type LSEMANTICS
            (f: ident) (ss os: list (Stream value))
            (Sem: sem_node G f ss os)
            {struct Sem}
-         : P_node f ss os.
+         : P_node f ss os
+    with sem_reset_ind2
+           (f: ident) (rs: Stream bool) (ss os: list (Stream value))
+           (Sem: sem_reset G f rs ss os)
+           {struct Sem}
+         : P_reset f rs ss os.
     Proof.
-      - destruct Sem.
-        + apply ConstCase.
-        + apply VarCase; auto.
-        + eapply UnopCase; eauto.
-        + eapply BinopCase; eauto.
+      - destruct Sem; eauto.
         + eapply FbyCase; eauto; clear H2; SolveForall.
         + eapply WhenCase; eauto; clear H2; SolveForall.
         + eapply MergeCase; eauto; clear H3; SolveForall.
         + eapply IteCase; eauto; clear H2; SolveForall.
         + eapply AppCase; eauto; clear H1; SolveForall.
+        + eapply ResetCase; eauto; clear H2; SolveForall.
       - destruct Sem.
         eapply Equation with (ss:=ss); eauto; clear H1; SolveForall.
       - destruct Sem.
         eapply Node; eauto.
         SolveForall.
+      - destruct Sem as [???? Sem].
+        eapply Reset; eauto.
     Qed.
 
   End sem_exp_ind2.
@@ -382,6 +426,6 @@ Module LSemanticsFun
        (Import Op    : OPERATORS)
        (Import OpAux : OPERATORS_AUX Op)
        (Import Syn   : LSYNTAX   Ids Op)
-       <: LSEMANTICS Ids Op OpAux Syn.
+<: LSEMANTICS Ids Op OpAux Syn.
   Include LSEMANTICS Ids Op OpAux Syn.
 End LSemanticsFun.
