src/Lustre/LClocking.v
@@ -237,7 +237,21 @@ Module Type LCLOCKING
                     n.(n_in) (nclocksof es)
             /\ Forall2 (fun xtc a => inst_out b osub isub xtc = Some (snd a))
                        n.(n_out) anns) ->
-        wc_exp (Eapp f es anns).
+        wc_exp (Eapp f es None anns)
+
+    | wc_EappReset: forall f es r anns n,
+        Forall wc_exp es ->
+        DisjointIndexes (map nclockof es) ->
+        NoDup (indexes (map snd anns)) ->
+        find_node f G = Some n ->
+        (exists b isub osub,
+            Forall2 (fun xtc cke => inst_in b isub xtc = Some cke)
+                    n.(n_in) (nclocksof es)
+            /\ Forall2 (fun xtc a => inst_out b osub isub xtc = Some (snd a))
+                       n.(n_out) anns) ->
+        wc_exp r ->
+        (* TODO: clock of r *)
+        wc_exp (Eapp f es (Some r) anns).
 
     Definition wc_patvar (pvars: list ident) (ncks: list nclock)
                          (x: ident) (sck: sclock) : Prop :=
@@ -362,7 +376,23 @@ Module Type LCLOCKING
                     n.(n_in) (nclocksof es)
             /\ Forall2 (fun xtc a => inst_out b osub isub xtc = Some (snd a))
                        n.(n_out) anns) ->
-        P (Eapp f es anns).
+        P (Eapp f es None anns).
+
+    Hypothesis EappResetCase:
+      forall f es r anns n,
+        Forall (wc_exp G vars) es ->
+        DisjointIndexes (map nclockof es) ->
+        NoDup (indexes (map snd anns)) ->
+        Forall P es ->
+        find_node f G = Some n ->
+        (exists b isub osub,
+            Forall2 (fun xtc cke => inst_in b isub xtc = Some cke)
+                    n.(n_in) (nclocksof es)
+            /\ Forall2 (fun xtc a => inst_out b osub isub xtc = Some (snd a))
+                       n.(n_out) anns) ->
+        wc_exp G vars r ->
+        P r ->
+        P (Eapp f es (Some r) anns).
 
     Fixpoint wc_exp_ind2 (e: exp) (H: wc_exp G vars e) {struct H} : P e.
     Proof.
@@ -379,6 +409,8 @@ Module Type LCLOCKING
         clear H3. induction H0; auto.
         clear H4. induction H1; auto.
       - eapply EappCase; eauto.
+        clear H0 H1 H2 H3. induction H; eauto.
+      - eapply EappResetCase; eauto.
         clear H0 H1 H2 H3. induction H; eauto.
     Qed.
 
